@prefix dct: <http://purl.org/dc/terms/> .
@prefix dcat: <http://www.w3.org/ns/dcat#> .
@prefix ids: <https://w3id.org/ids/core/> .
@prefix idsm: <https://w3id.org/ids/metamodel/> .
@prefix owl: <http://www.w3.org/2002/07/owl#> .
@prefix rdfs: <http://www.w3.org/2000/01/rdf-schema#> .
@prefix xsd: <http://www.w3.org/2001/XMLSchema#> .

# Classes
# -------

ids:Content a owl:Class;
    idsm:abstract true;
    # TODO, discuss: rdfs:subClassOf dcat:Dataset or adms:Asset?
    rdfs:label "Content"@en;
    rdfs:comment "Abstract content of a Resource that is encoded according to a Representation and optionally materialized as an Artifact."@en;
    idsm:validation [
        idsm:forProperty ids:contentType;
        idsm:relationType idsm:OneToMany;
    ];    
    idsm:validation [
        idsm:forProperty ids:representation;
        idsm:relationType idsm:OneToMany;
    ].

# Properties
# ----------

ids:representation a owl:ObjectProperty;
    rdfs:label "representation"@en;    
    rdfs:domain ids:Content;
    rdfs:range ids:Representation;
    rdfs:comment "Reference to a Representation of the abstract Resource Content."@en.

ids:part a owl:ObjectProperty;
    # TODO, dicuss: rdfs:subPropertyOf dct:hasPart or adms:includedAsset or some upper-level ontology property?
    rdfs:label "part"@en;
    idsm:labelPluralForm "parts"@en;
    rdfs:domain ids:Content;
    rdfs:range ids:Content;
    rdfs:comment "Reference to Content (physically or logically) included in given Content supporting definition of part-whole hierarchies."@en .

ids:sample a owl:ObjectProperty;
    # TODO, dicuss: rdfs:subPropertyOf adms:sample or ..?
    rdfs:label "sample"@en;
    rdfs:domain ids:Content;
    # What is the range - since real data, not metadata?
    rdfs:range rdfs:Resource;
    rdfs:comment "Sample Content instance."@en.

ids:variant a owl:ObjectProperty;
    # TODO, dicuss: rdfs:subPropertyOf adms:translation or ..?    
    idsm:abstract true ;
    rdfs:label "variant"@en;
    rdfs:domain ids:Content;
    rdfs:range ids:Content;
    rdfs:comment "Equivalent variant of given Content, e.g. a translation."@en.

# TODO, consider versioning properties, e.g. dcterms:date 
# TODO, consider versioning predicates,  e.g. adms:prev, adms:next, adms:last, dcterms:isReplacedBy
# TODO, consider annotation properties, e.g. dcterms:abstract, dcterms:description

# TODO, clarify whether we need "member" vs. "part"
#    rdfs:subPropertyOf ids:part;
#    rdfs:label "member"@en;
#    rdfs:domain ids:Collection;
#    rdfs:range ids:Content;
#    rdfs:comment "Reference to a Collection member."@en.

ids:contentType a owl:ObjectProperty;
    # TODO, discuss: rdfs:subPropertyOf dct:hasPart dct:type?
    rdfs:label "content type"@en;    
    rdfs:domain ids:Content;
    rdfs:range ids:ContentType;
    rdfs:comment "Reference to the abstract nature (type) of the Content."@en.

