@prefix owl: <http://www.w3.org/2002/07/owl#> .
@prefix rdfs: <http://www.w3.org/2000/01/rdf-schema#> .
@prefix xsd: <http://www.w3.org/2001/XMLSchema#> .
@prefix dct: <http://purl.org/dc/terms/> .
@prefix dcat: <http://www.w3.org/ns/dcat#> .
@prefix ids: <https://w3id.org/ids/core/> .
@prefix idsm: <https://w3id.org/ids/metamodel/> .

# Classes
# -------

ids:DataAsset
    a owl:Class;
    rdfs:subClassOf ids:Resource;    
    rdfs:label "DataAsset"@en;
    rdfs:comment "Resource exchanged via Data Endpoints of the Connector. Data Assets are expected to be focused, homogeneous, and consistent over time with regard to granularity, coverage, context, data structure, and conceptual classification"@en ;
    idsm:validation [
        idsm:forProperty ids:coversTemporal;
        idsm:relationType idsm:OneToMany;
    ];
    idsm:validation [
        idsm:forProperty ids:coversSpatial;
        idsm:relationType idsm:OneToMany;
    ];
    idsm:validation [
        idsm:forProperty ids:theme;
        idsm:relationType idsm:OneToMany;
    ];
    idsm:validation [
        idsm:forProperty ids:keyword;
        idsm:relationType idsm:OneToMany;
    ];
    idsm:validation [
        idsm:forProperty ids:coversLanguage;
        idsm:relationType idsm:OneToMany;
    ];
    idsm:validation [
        idsm:forProperty ids:retrievableBy;
        idsm:relationType idsm:OneToMany;
    ].

# Properties
# ----------

ids:theme a owl:ObjectProperty;
    rdfs:subPropertyOf dcat:theme;
    rdfs:label "theme"@en;
    idsm:labelPluralForm "themes"@en;
    rdfs:domain ids:DataAsset;
    rdfs:range ids:ContentCategory;
    rdfs:comment "Links to a taxonomy entry point that categorizes content-related coverage of the DataAsset."@en.

ids:keyword a owl:DatatypeProperty;
    rdfs:subPropertyOf dcat:keyword;
    rdfs:label "keyword"@en;
    idsm:labelPluralForm "keywords"@en;
    rdfs:domain ids:DataAsset;
    rdfs:range rdfs:Literal;
    rdfs:comment "Links to an item in a flat list of controlled keywords that describe content-related coverage of the DataAsset."@en.

# check naming and purpose <-> Context?
ids:coversTemporal a owl:ObjectProperty;
    rdfs:subPropertyOf dct:temporal;
    rdfs:label "coversTemporal"@en;
    rdfs:domain ids:DataAsset;
    rdfs:range ids:TemporalEntity;
    rdfs:comment "Temporal period or instance covered by the DataAsset."@en.

ids:coversSpatial a owl:ObjectProperty;
    rdfs:subPropertyOf dct:spatial;
    rdfs:label "coversSpatial"@en;
    rdfs:domain ids:DataAsset;
    rdfs:range ids:SpatialEntity;
    rdfs:comment "Spatial location covered by the DataAsset."@en.

