@prefix owl: <http://www.w3.org/2002/07/owl#> .
@prefix rdfs: <http://www.w3.org/2000/01/rdf-schema#> .
@prefix dct: <http://purl.org/dc/terms/> .
@prefix dcat: <http://www.w3.org/ns/dcat#> .
@prefix rdf: <http://www.w3.org/1999/02/22-rdf-syntax-ns#> .
@prefix xsd: <http://www.w3.org/2001/XMLSchema#> .
@prefix ids: <https://w3id.org/ids/core/> .
@prefix idsm: <https://w3id.org/ids/metamodel/> .

# Classes
# -------

ids:Representation
    a owl:Class ;
    #  TODO, discuss: rdfs:subClassOf dcat:Distribution / adms:AssetDistribution or ..?
    rdfs:label "Representation"@en;
    rdfs:comment "Serialization, i.e. syntactic description of Content."@en.

# Properties
# ----------

ids:artifact
    a owl:ObjectProperty ;    
    rdfs:domain ids:Representation ;
    rdfs:range ids:Artifact ;
    rdfs:label "artifact"@en ;
    rdfs:comment "Reference to a materialization of this Resource Representation (Artifact)."@en.

# TODO, clarify usage - there is no restriction on range!
#ids:format rdfs:subPropertyOf dct:format;
#    a owl:DatatypeProperty;
#    rdfs:domain ids:Representation;
#    rdfs:range xsd:string;
#    rdfs:label "format"@en;
#    rdfs:comment "The file format of the Representation. ids:mediaType SHOULD be used if the type of the distribution is defined by IANA."@en.

# ids:dataType xsd:Integer

ids:dataType
    a owl:ObjectProperty ;        
    rdfs:domain ids:Representation ;
    rdfs:range xsd:anyURI;
    rdfs:label "datatype"@en ;
    rdfs:comment "Reference to Datatype this Representation confirms to (defined in terms of a schema language)."@en;
    rdfs:seeAlso <http://www.ddialliance.org/Specification/DDI-CV/DataType_1.0.html> .
    
ids:mediaType
    a owl:ObjectProperty ;
    # TODO, consider further types: dcterms:FileFormat/dcterms:MediaType etc
    rdfs:subPropertyOf dcat:mediaType ;    
    rdfs:domain ids:Representation ;
    rdfs:range ids:MediaType ;
    rdfs:label "mediaType"@en ;
    rdfs:comment "Media Type of the Representation."@en.

ids:conformsToStandard
    a owl:DatatypeProperty ;
    rdfs:subPropertyOf dct:conformsTo ;
    rdfs:domain ids:Representation;
    rdfs:range xsd:anyURI;
    rdfs:label "conforms to standard"@en;
    rdfs:comment "An established standard the Representation conforms to."@en.

ids:schemaLink a owl:DatatypeProperty;
    rdfs:domain ids:Representation;
    rdfs:range xsd:anyURI;
    rdfs:label "Schema link"@en;
    rdfs:comment "Link to a document that contains additional information like class and type descriptions or integrity constraints describing the Representation's structure."@en.

ids:schemaDefinition a owl:DatatypeProperty;
    rdfs:domain ids:Representation;
    rdfs:range xsd:string;
    rdfs:label "Schema definition"@en;
    rdfs:comment "Formal definition of the Representation's structure provided inline, matching its data and media type (e.g, JSON Schema or XSD)."@en.
