@prefix dct: <http://purl.org/dc/terms/> .
@prefix dcat: <http://www.w3.org/ns/dcat#> .
@prefix ids: <https://w3id.org/ids/core/> .
@prefix idsm: <https://w3id.org/ids/metamodel/> .
@prefix owl: <http://www.w3.org/2002/07/owl#> .
@prefix rdf:   <http://www.w3.org/1999/02/22-rdf-syntax-ns#> .
@prefix rdfs: <http://www.w3.org/2000/01/rdf-schema#> .
@prefix xsd: <http://www.w3.org/2001/XMLSchema#> .

# Classes
# -------

ids:Resource
    a owl:Class;
    # rdfs:subClassOf ids:Identifiable - not needed, identity / reference supported via node URI, prevent usage of a blank node!
    rdfs:subClassOf ids:Described, ids:DigitalContent, dcat:Dataset, ids:ManagedEntity; 
    idsm:abstract true;
    rdfs:label "Resource"@en ;
    rdfs:comment "Superclass of digital Resources that are formalized in Representations and optionally materialized as Artifacts. The Resource's content is exposed via defined Interfaces at various protocol Endpoints."@en;    
    rdfs:seeAlso <https://www.w3.org/TR/vocab-dcat/#class-dataset>;
    idsm:validation [
        idsm:forProperty ids:interface;
        idsm:relationType idsm:OneToMany;
    ].

# Properties
# ------------

# Selection based on DCAT-AP 1.1 mandatory and recommended properties for dcat:Dataset
#
# title/description inherited from Described

# distribution cardinality in DCAT-AP: 0..n
ids:representation
    a owl:ObjectProperty;
    rdfs:subPropertyOf dcat:distribution ; # Links to non-materialized part of Distribution
    rdfs:label "representation"@en;
    rdfs:domain ids:Resource;
    rdfs:range ids:Representation;
    rdfs:comment "Reference to a Representation of the Resource."@en.

ids:defaultRepresentation
    a owl:ObjectProperty;
    rdfs:subPropertyOf ids:representation ;
    rdfs:label "Default representation"@en;
    rdfs:domain ids:Resource;
    rdfs:range ids:Representation;
    rdfs:comment "Reference to the default Representation of a Resource."@en.

ids:resourceInterface
    a owl:ObjectProperty;# Renamed from "interface" to be distinguished from a Software's programming interface
    rdfs:label "resource interface"@en;
    rdfs:domain ids:Resource;
    rdfs:range ids:Interface;
    rdfs:comment "Reference to the Interface defining Operations supported by the Resource."@en.

#ids:licence -> moved into Contract Offer
#    a owl:ObjectProperty ;
#    rdfs:subPropertyOf dct:licence ;
#    rdfs:domain ids:Resource ;
#    rdfs:range ids:License ;
#    rdfs:label "license"@en;
#    rdfs:comment "Reference to License(s) regulating the general usage of the Resource."@en.

# compare dct:rights etc.
ids:contractOffer
    a owl:ObjectProperty;
    rdfs:domain ids:Resource;
    rdfs:range ids:ContractOffer;
    rdfs:label "contract offer"@en;
    rdfs:comment "Reference to a Contract Offer defining the authorized use of the Resource."@en.

ids:publisher
    a owl:ObjectProperty ;
    rdfs:subPropertyOf dct:publisher ;
    rdfs:domain ids:Resource ;
    rdfs:range ids:Agent ;
    rdfs:label "publisher"@en;
    rdfs:comment "The publisher of the resource (which may differ from the sovereign)."@en.

ids:sovereign
    a owl:ObjectProperty ;
    rdfs:domain ids:Resource ;
    rdfs:range ids:Agent ;
    rdfs:label "sovereign"@en;
    rdfs:comment "The 'owner', i.e. sovergin of the data."@en.

ids:sample a owl:ObjectProperty;
    # dicuss: rdfs:subPropertyOf and range
    rdfs:label "sample"@en;    
    rdfs:domain ids:Resource;
    rdfs:range ids:Resource;# Web-retrievable or inline content
    rdfs:comment "Sample Resource instance."@en.

ids:variant a owl:ObjectProperty;
    # dicuss: rdfs:subPropertyOf adms:translation or ..?    
    idsm:abstract true ;
    rdfs:label "variant"@en;
    rdfs:domain ids:Resource;
    rdfs:range ids:Resource;
    rdfs:comment "(Equivalent) variant of given Resource, e.g. a translation."@en.

