@prefix dct: <http://purl.org/dc/terms/> .
@prefix dcat: <http://www.w3.org/ns/dcat#> .
@prefix ids: <https://w3id.org/ids/core/> .
@prefix idsm: <https://w3id.org/ids/metamodel/> .
@prefix owl: <http://www.w3.org/2002/07/owl#> .
@prefix rdf:   <http://www.w3.org/1999/02/22-rdf-syntax-ns#> .
@prefix rdfs: <http://www.w3.org/2000/01/rdf-schema#> .
@prefix xsd: <http://www.w3.org/2001/XMLSchema#> .

# Classes
# -------

ids:Resource a owl:Class;
    rdfs:subClassOf ids:Identifiable, ids:DigitalContent, dcat:Dataset, ids:ManagedEntity;
    rdfs:subClassOf
    [
      rdf:type          owl:Restriction ;
      owl:onProperty    ids:identifier ;
      owl:allValuesForm   ids:ResourceIdentifier;
    ];
    idsm:abstract true;
    rdfs:label "Resource"@en ;
    rdfs:comment "Superclass of digital Resources that is encoded according to a Representation and optionally materialized as an Artifact."@en;    
    rdfs:seeAlso <https://www.w3.org/TR/vocab-dcat/#class-dataset>.

# Properties
# ------------

ids:representation a owl:ObjectProperty;
    rdfs:label "representation"@en;    
    rdfs:domain ids:Resource;
    rdfs:range ids:Representation;
    rdfs:comment "Reference to a Representation of the abstract Resource."@en.

ids:interface a owl:ObjectProperty;
    rdfs:label "interface"@en;
    rdfs:domain ids:Resource;
    rdfs:range ids:Interface;
    rdfs:comment "Reference to the Interface defining Operations supported by the Resource."@en.

ids:licence
    a owl:ObjectProperty ;
    rdfs:subPropertyOf dct:licence ;
    rdfs:domain ids:Resource ;
    rdfs:range ids:License ;
    rdfs:label "license"@en;
    rdfs:comment "Reference to License(s) regulating the general usage of the Resource."@en.

# compare dct:rights etc.
ids:contract
    a owl:ObjectProperty;
    rdfs:domain ids:Resource;
    rdfs:range ids:Contract;
    rdfs:label "contract"@en;
    rdfs:comment "Reference to Contract(s) regulating a particular usage of the Resource."@en.

ids:sovereign
    a owl:ObjectProperty ;
    rdfs:subPropertyOf dct:publisher ;
    rdfs:domain ids:Resource ;
    rdfs:range ids:Agent ;
    rdfs:label "sovereign"@en;
    rdfs:comment "The original issuer, i.e. sovergin of the data."@en.

ids:sample a owl:ObjectProperty;
    # dicuss: rdfs:subPropertyOf and range
    rdfs:label "sample"@en;    
    rdfs:domain ids:Resource;    
    rdfs:range rdfs:Resource;
    rdfs:comment "Sample Resource instance."@en.

ids:variant a owl:ObjectProperty;
    # dicuss: rdfs:subPropertyOf adms:translation or ..?    
    idsm:abstract true ;
    rdfs:label "variant"@en;
    rdfs:domain ids:Resource;
    rdfs:range ids:Resource;
    rdfs:comment "Equivalent variant of given Resource, e.g. a translation."@en.
