@prefix owl: <http://www.w3.org/2002/07/owl#> .
@prefix rdfs: <http://www.w3.org/2000/01/rdf-schema#> .
@prefix dct: <http://purl.org/dc/terms/> .
@prefix dcat: <http://www.w3.org/ns/dcat#> .
@prefix rdf: <http://www.w3.org/1999/02/22-rdf-syntax-ns#> .
@prefix xsd: <http://www.w3.org/2001/XMLSchema#> .
@prefix ids: <https://w3id.org/ids/core/> .
@prefix idsm: <https://w3id.org/ids/metamodel/> .

# Classes
# -------

ids:Serialization
    a owl:Class ;    
    rdfs:label "Serialization"@en;
    rdfs:comment "Serialization, i.e. syntactic description of a Digital Content."@en.

# Properties
# ----------

ids:schemaReference a owl:DatatypeProperty;
    rdfs:domain ids:Serialization;
    rdfs:range xsd:anyURI;
    rdfs:label "schema reference"@en;
    rdfs:comment "Reference to Datatype this Serialization conforms to (defined in terms of a schema language)."@en;
    rdfs:seeAlso <http://www.ddialliance.org/Specification/DDI-CV/DataType_1.0.html> .

ids:schemaInline a owl:DatatypeProperty;
    rdfs:domain ids:Serialization;
    rdfs:range xsd:string;
    rdfs:label "schema inline"@en;
    rdfs:comment "Formal definition of the Representation's structure provided inline, matching its data and media type (e.g, JSON Schema or XSD)."@en.
