@prefix owl: <http://www.w3.org/2002/07/owl#> .
@prefix rdfs: <http://www.w3.org/2000/01/rdf-schema#> .
@prefix xsd: <http://www.w3.org/2001/XMLSchema#> .
@prefix dct: <http://purl.org/dc/terms/> .
@prefix dcat: <http://www.w3.org/ns/dcat#> .
@prefix ids: <https://w3id.org/ids/core/> .
@prefix idsm: <https://w3id.org/ids/metamodel/> .

# Classes
# -------

ids:DataAsset rdfs:subClassOf ids:ManagedEntity;
    rdfs:subClassOf ids:Resource;
    rdfs:subClassOf dcat:Dataset;
    a owl:Class;
    rdfs:label "DataAsset"@en;
    rdfs:comment "Class describing data on the Industrial Dataspace. May be a data offering, data that is in the state of being transfered or an aggregation of multiple other dataassets."@en;
    idsm:validation [
        idsm:forProperty ids:coversTemporal;
        idsm:relationType idsm:OneToMany;
    ];
    idsm:validation [
        idsm:forProperty ids:coversSpatial;
        idsm:relationType idsm:OneToMany;
    ];
    idsm:validation [
        idsm:forProperty ids:contentCategory;
        idsm:relationType idsm:OneToMany;
    ];
    idsm:validation [
        idsm:forProperty ids:kind;
        idsm:relationType idsm:OneToMany;
    ];
    idsm:validation [
        idsm:forProperty ids:coversLanguage;
        idsm:relationType idsm:OneToMany;
    ].

# Properties
# ----------

ids:kind a owl:ObjectProperty;
    rdfs:label "kind"@en;
    ids:labelPluralForm "kinds"@en;
    rdfs:domain ids:DataAsset;
    rdfs:range ids:Kind;
    rdfs:comment "Describes the DataAsset's Kind."@en.

ids:version rdfs:subPropertyOf dct:hasVersion;
    a owl:DatatypeProperty;
    rdfs:label "version"@en;
    rdfs:domain ids:DataAsset;
    rdfs:range xsd:string;
    rdfs:comment "Version identifier of the InfrastructureComponent."@en.

ids:coversTemporal a owl:ObjectProperty;
    rdfs:subPropertyOf dct:temporal;
    rdfs:label "coversTemporal"@en;
    rdfs:domain ids:DataAsset;
    rdfs:range ids:TemporalEntity;
    rdfs:comment "Temporal period or instance covered by the DataAsset."@en.

ids:coversSpatial a owl:ObjectProperty;
    rdfs:subPropertyOf dct:spatial;
    rdfs:label "coversSpatial"@en;
    rdfs:domain ids:DataAsset;
    rdfs:range ids:SpatialEntity;
    rdfs:comment "Spatial location covered by the DataAsset."@en.

ids:coversLanguage a owl:ObjectProperty;
    rdfs:subPropertyOf dct:language;
    rdfs:label "coversLanguage"@en;
    ids:labelPluralForm "coversLanguages"@en;
    rdfs:domain ids:DataAsset;
    rdfs:range ids:Language;
    ids:refByURI true;
    rdfs:comment "States the languages that are used by the content of the DataAsset."@en.

ids:origin a owl:DatatypeProperty;
    rdfs:label "origin"@en;
    rdfs:domain ids:DataAsset;
    rdfs:range xsd:anyURI;
    rdfs:comment "Link to the original resource from which the content of the DataAsset has been derived or is a copy of."@en.

ids:contentCategory a owl:ObjectProperty;
    rdfs:subPropertyOf dcat:theme;
    rdfs:label "contentCategory"@en;
    ids:labelPluralForm "contentCategories"@en;
    rdfs:domain ids:DataAsset;
    rdfs:range ids:ContentCategory;
    rdfs:comment "Links to a taxonomy entry point that categorizes content-related coverage of the DataAsset."@en.

ids:keyword a owl:DatatypeProperty;
    rdfs:subPropertyOf dcat:theme;
    rdfs:label "keyword"@en;
    ids:labelPluralForm "keywords"@en;
    rdfs:domain ids:DataAsset;
    rdfs:range xsd:anyURI;
    rdfs:comment "Links to an item in a flat list of controlled keywords that describe content-related coverage of the DataAsset."@en.

ids:contract a owl:ObjectProperty;
    rdfs:domain ids:DataAsset;
    rdfs:range ids:Contract;
    rdfs:label "contract"@en;
    rdfs:comment "The Contract regulating usage of the DataAsset."@en.
