@prefix idsm: <https://w3id.org/ids/metamodel/> .
@prefix owl: <http://www.w3.org/2002/07/owl#> .
@prefix rdf: <http://www.w3.org/1999/02/22-rdf-syntax-ns#> .
@prefix rdfs: <http://www.w3.org/2000/01/rdf-schema#> .
@prefix skos: <http://www.w3.org/2004/02/skos/core#> .
@prefix xsd: <http://www.w3.org/2001/XMLSchema#> .

# Properties
# ----------

idsm:abstract a owl:DatatypeProperty;
    rdfs:label "isAbstract"@en;
    rdfs:domain owl:Class;
    rdfs:range xsd:boolean;
    rdfs:comment "Abstract concept, i.e. it is expected there are no instantiations of this class, but concrete subclasses."@en.

idsm:labelPluralForm a owl:ObjectProperty;
    rdfs:subPropertyOf skos:prefLabel;
	rdfs:label "labelPluralForm"@en;
	rdfs:domain rdfs:Resource;
	rdfs:range rdf:PlainLiteral;
    rdfs:comment "The preferred lexical label for a resource, in plural form in a given language."@en.

idsm:explanation a owl:DatatypeProperty;
    rdfs:label "explanation"@en;
    rdfs:domain owl:Class;
    rdfs:range xsd:string;
    rdfs:comment "Verbose description of motivations and design decisions underlying the concept."@en.

idsm:competencyQuestion a owl:DatatypeProperty;
    rdfs:label "competency question"@en;
    rdfs:domain owl:Class;
    rdfs:range xsd:string;
    rdfs:comment "Single 'competency question' the concept is intended to address."@en ;
    rdfs:seeAlso <https://protege.stanford.edu/publications/ontology_development/ontology101-noy-mcguinness.html#Step1> ;
    .

idsm:constantIdentifier a owl:DatatypeProperty;
    rdfs:label "constantIdentifier"@en;
    rdfs:range xsd:string;
    rdfs:comment "Defines the identifier of an individual when represented as an enumeration type in the target programming language."@en.

idsm:referenceByUrl a owl:DatatypeProperty;
    rdfs:label "Reference by URL"@en;
    rdfs:domain owl:Class;
    rdfs:range xsd:boolean;
    rdfs:comment "States that a reference to a class should not be implemented by a local in-memory reference but as a URL addressing the remote instance."@en.