@prefix owl: <http://www.w3.org/2002/07/owl#> .
@prefix rdf: <http://www.w3.org/1999/02/22-rdf-syntax-ns#> .
@prefix rdfs: <http://www.w3.org/2000/01/rdf-schema#> .
@prefix xsd: <http://www.w3.org/2001/XMLSchema#> .
@prefix dct: <http://purl.org/dc/terms/> .
@prefix ids: <https://w3id.org/ids/core/> .
@prefix idsm: <https://w3id.org/ids/metamodel/> .

# Classes
# -------

ids:Parameter a owl:Class;
#    rdfs:subClassOf ids:Named, ids:DigitalContent;
    rdfs:subClassOf ids:DigitalContent;
    rdfs:label "Parameter"@en ;
    rdfs:comment "Named slot of an Interface Operation i.e., an input, output or fault (exception)."@en;
    idsm:abstract true;
    idsm:validation [
        idsm:forProperty ids:paramLabel;
        idsm:relationType idsm:OneToMany;
    ];
    idsm:validation [
        idsm:forProperty ids:paramDescription;
        idsm:relationType idsm:OneToMany;
    ].

# Properties for describing a Parameter
# -------------------------------------

ids:paramLabel rdfs:subPropertyOf rdfs:label;
    a owl:DatatypeProperty;
    rdfs:domain ids:Parameter;
    rdfs:range rdf:PlainLiteral;
    rdfs:label "paramLabel"@en;
    idsm:labelPluralForm "paramLabels"@en;
    rdfs:comment "Freetext label of the Parameter as it should be shown in public indexes."@en.

ids:paramName rdfs:subPropertyOf dct:identifier;
    a owl:DatatypeProperty;
    rdfs:domain ids:Parameter;
    rdfs:range xsd:string;
    rdfs:label "paramName"@en;    
    rdfs:comment "Name of the Parameter as it must be used in service requests."@en.

ids:paramDescription rdfs:subPropertyOf dct:description;
    a owl:DatatypeProperty;
    rdfs:domain ids:Parameter;
    rdfs:range rdf:PlainLiteral;
    rdfs:label "paramDescription"@en;
    idsm:labelPluralForm "paramDescriptions"@en;
    rdfs:comment "Freetext description of the Parameter as it should be shown in public indexes."@en.

ids:dataType a owl:ObjectProperty;
    rdfs:domain ids:Parameter;
    rdfs:range ids:ParameterDataType;
    rdfs:label "dataType"@en;
    rdfs:comment "Indicates the datatype of the Parameter."@en.

ids:refersTo a owl:ObjectProperty;
    rdfs:domain ids:Parameter;
    rdfs:range ids:Resource;
    rdfs:label "refersTo"@en;
    rdfs:comment "Indicates the Resource to which the Parameter refers to."@en.

ids:covers a owl:ObjectProperty;
    rdfs:domain ids:Parameter;
    rdfs:range ids:Representation;
    rdfs:label "covers"@en;
    rdfs:comment "The Representation consumed or returned by a Parameter."@en.
