@prefix owl: <http://www.w3.org/2002/07/owl#> .
@prefix dct: <http://purl.org/dc/terms/> .
@prefix rdfs: <http://www.w3.org/2000/01/rdf-schema#> .
@prefix prov: <http://www.w3.org/ns/prov#> .
@prefix rdf: <http://www.w3.org/1999/02/22-rdf-syntax-ns#> .
@prefix xsd: <http://www.w3.org/2001/XMLSchema#> .
@prefix ids: <https://w3id.org/ids/core> .

# Classes
# -------

ids:EntityWithLifecycle a owl:Class;
    ids:isAbstract true;
    rdfs:label "EntityWithLifecycle"@en ;
    rdfs:comment "The class of all individuals that are subject of a lifecycle which needs to be tracked.";
    ids:validation [
        ids:forProperty ids:lifecycleActivity;
        ids:relationType ids:OneToMany;
    ];
    ids:validation [
        ids:forProperty ids:entityName;
        ids:relationType ids:OneToMany;
        ids:constraint ids:NotNull;
    ];
    ids:validation [
        ids:forProperty ids:entityDescription;
        ids:relationType ids:OneToMany;
    ].

ids:InfrastructureComponent rdfs:subClassOf ids:EntityWithLifecycle;
    a owl:Class;
    ids:isAbstract true;
    rdfs:label "InfrastructureComponent"@en ;
    rdfs:comment "The class of all infrastructure components of the IDS.";
    ids:validation [
        ids:forProperty ids:technicalResponsibility;
        ids:constraint ids:NotNull;
    ];
    ids:validation [
        ids:forProperty ids:contentResponsibility;
        ids:constraint ids:NotNull;
    ];
    ids:validation [
        ids:forProperty ids:supportedIMVersion;
        ids:relationType ids:OneToMany;
    ].

# Properties of InfrastructureComponent
# -------------------------------------

ids:maintainer a owl:ObjectProperty;
    rdfs:label "maintainer"@en;
    rdfs:domain ids:InfrastructureComponent;
    rdfs:range ids:Participant;
    ids:refByURI true;
    rdfs:comment "Participant responsible for maintaining the InfrastructureComponent."@en.

ids:contentResponsibility a owl:ObjectProperty;
    rdfs:label "contentResponsibility"@en;
    rdfs:domain ids:InfrastructureComponent;
    rdfs:range ids:Participant;
    ids:refByURI true;
    rdfs:comment "Participant responsible for content provided by the InfrastructureComponent."@en.

ids:technicalResponsibility a owl:ObjectProperty;
    rdfs:label "technicalResponsibility"@en;
    rdfs:domain ids:InfrastructureComponent;
    rdfs:range ids:Participant;
    ids:refByURI true;
    rdfs:comment "Participant responsible for technical operation of the InfrastructureComponent."@en.

ids:physicalLocation a owl:ObjectProperty;
    rdfs:label "physicalLocation"@en;
    rdfs:domain ids:InfrastructureComponent;
    rdfs:range ids:Location;
    rdfs:comment "The location where the Connector is physically deployed."@en.

ids:supportedIMVersion a owl:DatatypeProperty;
    rdfs:label "supportedIMVersion"@en;
    ids:labelPluralForm "supportedIMVersions"@en;
    rdfs:domain ids:InfrastructureComponent;
    rdfs:range xsd:anyURI;
    rdfs:comment "The versions of the Information Model that are supported by the InfrastructureComponent."@en.

# Properties of EntityWithLifecycle
# -------------------------------------

ids:entityName rdfs:subPropertyOf dct:title;
	a owl:DatatypeProperty;
	rdfs:domain ids:EntityWithLifecycle;
	rdfs:range rdf:PlainLiteral;
    rdfs:label "entityName"@en;
    ids:labelPluralForm "entityNames"@en;
	rdfs:comment "Name of the EntityWithLifecycle."@en.

ids:entityDescription rdfs:subPropertyOf dct:description;
	a owl:DatatypeProperty;
	rdfs:domain ids:EntityWithLifecycle;
	rdfs:range rdf:PlainLiteral;
	rdfs:label "entityDescription"@en;
	ids:labelPluralForm "entityDescriptions"@en;
	rdfs:comment "Freetext description of the EntityWithLifecycle.".

ids:generationActivity rdfs:subPropertyOf prov:wasGeneratedBy;
    a owl:ObjectProperty;
    rdfs:label "generationActivity"@en;
    rdfs:domain ids:EntityWithLifecycle;
    rdfs:range ids:CreationActivity;
    rdfs:comment "Activity that led to the generation of the InfrastructureComponent."@en.

ids:lifecycleActivity a owl:ObjectProperty;
    rdfs:label "lifecycleActivity"@en;
    ids:labelPluralForm "lifecycleActivities"@en;
    rdfs:domain ids:EntityWithLifecycle;
    rdfs:range ids:Activity;
    rdfs:comment "Activity that occurs during the lifecycle of the InfrastructureComponent."@en.