@prefix owl: <http://www.w3.org/2002/07/owl#> .
@prefix rdf:   <http://www.w3.org/1999/02/22-rdf-syntax-ns#> .
@prefix rdfs: <http://www.w3.org/2000/01/rdf-schema#> .
@prefix xsd: <http://www.w3.org/2001/XMLSchema#> .
@prefix dct: <http://purl.org/dc/terms/> .
@prefix ids: <https://w3id.org/ids/core/> .
@prefix idsm: <https://w3id.org/ids/metamodel/> .

# Classes
# -------

# Parameter subclasses serve the definition of restriction based on Parameter type
#
# Identification

# TODO, clarify how IdentifierParameter refers to/relates to Identifier (of Resource, Connector etc.)?
ids:IdentifierParameter
    rdfs:type owl:Class ;
    rdfs:subClassOf ids:Parameter ;
    rdfs:label "Identifier parameter"@en ; 
    rdfs:comment "Parameter for passing Resource identifiers as defined by a Resource Collection. The Resource identifier is unique and valid regardless of the actual extent, ordering, and view (filtering) of the Collection."@en .

ids:IndexParameter
    rdfs:type owl:Class ;
    rdfs:subClassOf ids:Parameter ;
    rdfs:label "Index parameter"@en ; 
    rdfs:comment "Parameter conveying the transient, positional identifier of a resource in the context of an ordered Collection. The resource index is temporarily unique and valid only with respect to the actual extent, ordering, and view (filtering) of the Collection."@en .

# Content
# adds reference to Content via "parameterContent" link, single cardinality per default ({1})
# explicit multiplicity marked by predicate parameterContentList ({1,n}), range of parameterContentList is Content #rdf:List
# content cardinalities along the predicate path:
#    1) input P parameterContent C {0,1}
#    3) input P parameterContentList C {0,n}
#    4) mandatoryInput P parameterContent C {1}
#    5) mandatoryInput P parameterContentList C {1,n}

ids:ContentParameter
    rdfs:type owl:Class ;
    rdfs:subClassOf ids:Parameter ;
    rdfs:label "Content parameter"@en ; 
    rdfs:comment "Parameter used to mediate a Content Representation, contrasted to parameters conveying auxiliary information."@en .

ids:parameterContent a owl:ObjectProperty;
    rdfs:domain ids:ContentParameter;
    rdfs:range ids:DigitalContent;
    rdfs:label "parameterContent"@en;
    rdfs:comment "Digital Content mediated by the Parameter."@en.

ids:parameterContentList a owl:ObjectProperty;
    rdfs:domain ids:ContentParameter;
    rdfs:range ids:DigitalContent;
    rdfs:label "parameter content list"@en;
    rdfs:comment "List of Digital Contents mediated by the Parameter."@en.

    
# Sorting

ids:SortOrderParameter
    rdfs:type owl:Class ;
    rdfs:subClassOf ids:Parameter ;
    rdfs:label "Sort order parameter"@en ;
    rdfs:comment "Parameter indicating the ordering of list items."@en .

ids:SortKeyParameter
    rdfs:type owl:Class ;
    rdfs:subClassOf ids:Parameter ;
    rdfs:label "Sort key parameter"@en ;
    rdfs:comment "Parameter indicating the key values underlying the sorting of items in a list."@en .

# Client-defined content view

# int
ids:OffsetParameter
    rdfs:type owl:Class ;
    rdfs:subClassOf ids:Parameter ;
    rdfs:label "Offset parameter"@en ;
    rdfs:comment "Parameter indicating the absolute offset (number of data elements to skip) within an ordered data Collection. Negative values are bounded at Collections's end (reverse index)."@en .

# nonNegativeInt > 0
ids:LimitParameter
    rdfs:type owl:Class ;
    rdfs:subClassOf ids:Parameter ;
    rdfs:label "Limit parameter"@en ;
    rdfs:comment "Parameter indicating the number of elements retrieved or provided at once within a paginated subset (page)."@en .

# Server-defined content view, pre-selected page size

# int, same as offset
ids:PageIndexParameter
    rdfs:type owl:Class ;
    rdfs:subClassOf ids:Index ;
    rdfs:label "Page index parameter"@en ; 
    rdfs:comment "Parameter conveying the transient, positional identifier of a content page within a server-defined pagination."@en .

# one of: first, last, previous, next
ids:PageReferenceParameter
    rdfs:type owl:Class ;
    rdfs:subClassOf ids:Index ;
    rdfs:label "Page reference parameter"@en ; 
    rdfs:comment "Parameter conveying the relative reference to a content page within a server-defined pagination."@en .


# Filtering

ids:FilterParameter
    rdfs:type owl:Class ;
    rdfs:subClassOf ids:Parameter ;
    rdfs:label "Filter parameter"@en ; 
    rdfs:comment "Parameter holding a filter expression (matcher) used to identify a matching subset of a collec­tion’s Resources."@en .
    # Extension of "Filter" parameter supporting hierarchical, nested data structures: SparqlPropertyPath, XPath, JSONPath, LDAP-Path etc.
    # LDAP-Path („Distinguished Name“, "DN")
    #   - https://docs.ldap.com/specs/rfc4514.txt
    #   - distinguished name (usually just shortened to “DN”) uniquely identifies an entry and describes its position in the DIT.
    # value "literal"^^ids:LDAPFilter; ""^^GraphPatternFilter -> custom datatype?

# Selection / extraction
    
ids:SelectorParameter
    rdfs:type owl:Class ;
    rdfs:subClassOf ids:Parameter ;
    rdfs:label "Selector parameter"@en ; 
    rdfs:comment "Parameter holding a selector expression used to retrieve a matching subset of a collection’s Resource contents."@en .
    # Examples: XQuery, SPARQL Construct/Select
