@prefix owl: <http://www.w3.org/2002/07/owl#> .
@prefix rdf: <http://www.w3.org/1999/02/22-rdf-syntax-ns#> .
@prefix rdfs: <http://www.w3.org/2000/01/rdf-schema#> .
@prefix xsd: <http://www.w3.org/2001/XMLSchema#> .
@prefix dct: <http://purl.org/dc/terms/> .
@prefix ids: <https://w3id.org/ids/core> .

# Classes
# -------

ids:ServiceInterface a owl:Class;
    rdfs:label "ServiceInterface"@en;
    rdfs:comment "Conceptualization of the interchange of digital artifacts as a set of uniform operations (interactions primitives)."@en.

ids:DataService a owl:Class;
    rdfs:label "DataService"@en;
    rdfs:comment "Class of Services to invoke an Interface."@en;
    ids:validation [
        ids:forProperty ids:binding;
        ids:constraint ids:NotNull;
    ].

ids:Operation a owl:Class;
    rdfs:label "Operation"@en;
    rdfs:comment "Building block of an Interface; describes the interaction by defining input, output and error parameters."@en;
    ids:validation [
        ids:forProperty ids:opLabel;
        ids:constraint ids:NotNull;
        ids:relationType ids:OneToMany;
    ];
    ids:validation [
        ids:forProperty ids:opDescription;
        ids:relationType ids:OneToMany;
        ids:constraint ids:NotNull;
    ];
    ids:validation [
        ids:forProperty ids:input;
        ids:relationType ids:OneToMany;
    ];
    ids:validation [
        ids:forProperty ids:output;
        ids:relationType ids:OneToMany;
    ].

ids:Parameter a owl:Class;
    rdfs:label "Parameter"@en ;
    rdfs:comment "Parameter to interact with an Interface, i.e., input, output or fault (exception)."@en;
    ids:isAbstract true;
    ids:validation [
        ids:forProperty ids:paramLabel;
        ids:relationType ids:OneToMany;
    ];
    ids:validation [
        ids:forProperty ids:paramDescription;
        ids:relationType ids:OneToMany;
    ];
    ids:validation [
        ids:forProperty ids:addKindSemantics;
        ids:relationType ids:OneToMany;
    ].

ids:ParameterGroup a owl:Class;
    rdfs:label "ParameterGroup"@en ;
    rdfs:comment "Class of grouped parameters, according to some grouping operator."@en;
    ids:validation [
        ids:forProperty ids:paramGroupingOperator;
        ids:relationType ids:NotNull;
    ];
    ids:validation [
        ids:forProperty ids:paramGroupMember;
        ids:relationType ids:OneToMany;
    ].

ids:InputParameter rdfs:subClassOf ids:Parameter;
    a owl:Class;
    rdfs:label "InputParameter"@en ;
    rdfs:comment "Input Parameter to control an Operation."@en.

ids:OutputParameter rdfs:subClassOf ids:Parameter;
    a owl:Class;
    rdfs:label "OutputParameter"@en ;
    rdfs:comment "Result of an Operation."@en.

ids:Fault rdfs:subClassOf ids:OutputParameter;
    a owl:Class;
    rdfs:label "Fault"@en ;
    rdfs:comment "Result on Operation failure."@en.

# Properties for describing an Interface
# --------------------------------------

ids:operation a owl:ObjectProperty;
    rdfs:domain ids:ServiceInterface;
    rdfs:range ids:Operation;
    rdfs:label "operation"@en;
    rdfs:comment "Declares the Operation to access a DataAsset."@en.

ids:implementer a owl:ObjectProperty;
    rdfs:domain ids:ServiceInterface;
    rdfs:range ids:DataService;
    rdfs:label "implementer"@en;
    rdfs:comment "Links to executable service that implements an Interface."@en.

ids:contract a owl:ObjectProperty;
    rdfs:domain ids:ServiceInterface;
    rdfs:range ids:Contract;
    rdfs:label "contract"@en;
    ids:labelPluralForm "contracts"@en;
    rdfs:comment "The Contract regulating usage of the Interface; in addition to the contracts that may be attached to the DataAsset"@en.

# Properties for describing a DataService
# ---------------------------------------

ids:binding a owl:ObjectProperty;
    rdfs:domain ids:DataService;
    rdfs:range ids:ProtocolBinding;
    rdfs:label "binding"@en;
    rdfs:comment "Links to the protocol bindings which define how to technically invoke the Service."@en.

# Properties for describing an Operation
# --------------------------------------

ids:input a owl:ObjectProperty;
    rdfs:domain ids:Operation;
    rdfs:range ids:InputParameter;
    rdfs:label "input"@en;
    ids:labelPluralForm "inputs"@en;
    rdfs:comment "Parameterizes the input of an Operation."@en.

ids:inputGroup a owl:ObjectProperty;
    rdfs:domain ids:Operation;
    rdfs:range ids:ParameterGroup;
    rdfs:label "inputGroup"@en;
    rdfs:comment "Parameterizes the input of an Operation with a predefined paramter group."@en.

ids:output a owl:ObjectProperty;
    rdfs:domain ids:Operation;
    rdfs:range ids:OutputParameter;
    rdfs:label "output"@en;
    ids:labelPluralForm "outputs"@en;
    rdfs:comment "Holds the result of an Operation."@en.

ids:fault a owl:ObjectProperty;
    rdfs:domain ids:Operation;
    rdfs:range ids:Fault;
    rdfs:label "fault"@en;
    ids:labelPluralForm "faults"@en;
    rdfs:comment "Holds information when an Operation has failed."@en.

ids:opLabel rdfs:subPropertyOf rdfs:label;
    a owl:DatatypeProperty;
    rdfs:domain ids:Operation;
    rdfs:range rdf:PlainLiteral;
    ids:labelPluralForm "opLabels"@en;
    rdfs:label "opLabel"@en;
    rdfs:comment "Freetext label of the Operation as it should be shown in public indexes."@en.

ids:opDescription rdfs:subPropertyOf dct:description;
    a owl:DatatypeProperty;
    rdfs:domain ids:Operation;
    rdfs:range rdf:PlainLiteral;
    ids:labelPluralForm "opDescriptions"@en;
    rdfs:label "opDescription"@en;
    rdfs:comment "Freetext description of the Operation as it should be shown in public indexes."@en.

ids:semantics a owl:ObjectProperty;
    rdfs:domain ids:Operation;
    rdfs:range ids:OperationSemantics;
    rdfs:label "semantics"@en;
    rdfs:comment "Semantic meaning of the Operation."@en.

# Properties for describing a Parameter
# -------------------------------------

ids:paramLabel rdfs:subPropertyOf rdfs:label;
    a owl:DatatypeProperty;
    rdfs:domain ids:Parameter;
    rdfs:range rdf:PlainLiteral;
    rdfs:label "paramLabel"@en;
    ids:labelPluralForm "paramLabels"@en;
    rdfs:comment "Freetext label of the Parameter as it should be shown in public indexes."@en.

ids:paramName rdfs:subPropertyOf dct:identifier;
    a owl:DatatypeProperty;
    rdfs:domain ids:Parameter;
    rdfs:range xsd:string;
    rdfs:label "paramName"@en;
    rdfs:comment "Name of the Parameter as it must be used in service requests."@en.

ids:paramDescription rdfs:subPropertyOf dct:description;
    a owl:DatatypeProperty;
    rdfs:domain ids:Parameter;
    rdfs:range rdf:PlainLiteral;
    rdfs:label "paramDescription"@en;
    ids:labelPluralForm "paramDescriptions"@en;
    rdfs:comment "Freetext description of the Parameter as it should be shown in public indexes."@en.

ids:dataType a owl:ObjectProperty;
    rdfs:domain ids:Parameter;
    rdfs:range ids:ParameterDataType;
    rdfs:label "dataType"@en;
    rdfs:comment "Indicates the datatype of the Parameter."@en.

ids:refersTo a owl:ObjectProperty;
    ids:refByURI true;
    rdfs:domain ids:Parameter;
    rdfs:range ids:Kind;
    rdfs:label "refersTo"@en;
    rdfs:comment "Indicates the Kind element to which the Parameter refers to."@en.

ids:addKindSemantics a owl:ObjectProperty;
    rdfs:domain ids:Parameter;
    rdfs:range ids:KindSemantics;
    rdfs:label "addKindSemantics"@en;
    rdfs:comment "Concretises semantics of a Parameter if it is more specific than the original Kind semantics."@en.

# Properties for describing a ParameterGroup
# ------------------------------------------

ids:paramGroupMember a owl:ObjectProperty;
    rdfs:domain ids:ParameterGroup;
    rdfs:range ids:Parameter;
    rdfs:label "paramGroupMember"@en;
    ids:labelPluralForm "paramGroupMembers"@en;
    rdfs:comment "Declares a member of a ParameterGroup."@en.

ids:paramGroupingOperator a owl:ObjectProperty;
    rdfs:domain ids:ParameterGroup;
    rdfs:range ids:ParameterGroupingOperator;
    rdfs:label "paramGroupingOperator"@en;
    rdfs:comment "Defines the operator that relates all members of the ParameterGroup."@en.