@prefix owl: <http://www.w3.org/2002/07/owl#> .
@prefix rdf: <http://www.w3.org/1999/02/22-rdf-syntax-ns#> .
@prefix rdfs: <http://www.w3.org/2000/01/rdf-schema#> .
@prefix xsd: <http://www.w3.org/2001/XMLSchema#> .
@prefix dct: <http://purl.org/dc/terms/> .

@prefix ids_int: <https://schema.industrialdataspace.org/interface/> .
@prefix ids_rel: <https://schema.iais.fraunhofer.de/ids/helper/relation/> .
@prefix ids_trans: <https://schema.iais.fraunhofer.de/ids/helper/transformation/> .
@prefix ids_doc: <https://schema.iais.fraunhofer.de/ids/helper/documentation/> .

# Classes
# -------

ids_int:ProtocolBinding a owl:Class;
    rdfs:label "ProtocolBinding"@en;
    rdfs:comment "Mapping of abstract operation signatures onto the concrete structures (e.g., HTTP headers or query parameters)."@en.

ids_int:ApiDocument a owl:Class;
    rdfs:label "ApiDocument"@en;
    rdfs:comment "Class of documents, fully and consistently describing an API, e.g., according to the OpenAPI specification."@en.


# Properties
# ----------

ids_int:uses a owl:ObjectProperty;
    rdfs:label "uses"@en;
    rdfs:domain ids_int:ProtocolBinding;
    rdfs:range ids_int:Protocol;
    rdfs:comment "Defines the Protocol used by the binding."@en.

ids_int:apiDocument a owl:ObjectProperty;
    rdfs:label "apiDocument"@en;
    rdfs:domain ids_int:ProtocolBinding;
    rdfs:range ids_int:ApiDocument;
    rdfs:comment "Document describing the API of the binding."@en.

ids_int:apiDocumentReference a owl:DatatypeProperty;
    rdfs:label "apiDocumentReference"@en;
    rdfs:domain ids_int:ProtocolBinding;
    rdfs:range xsd:string;
    rdfs:comment "References a structure inside the ApiDocument's content, e.g., a JSON path for OpenAPI documents."@en.

ids_int:apiDocumentType a owl:ObjectProperty;
    rdfs:label "apiDocumentType"@en;
    rdfs:domain ids_int:ApiDocument;
    rdfs:range ids_int:ApiDocumentType;
    rdfs:comment "Type of the ApiDocument."@en.

ids_int:content a owl:DatatypeProperty;
    rdfs:label "content"@en;
    rdfs:domain ids_int:ApiDocument;
    rdfs:range xsd:string;
    rdfs:comment "Textual representation of an API description, e.g., the OpenAPI JSON structure."@en.