@prefix owl: <http://www.w3.org/2002/07/owl#> .
@prefix rdfs: <http://www.w3.org/2000/01/rdf-schema#> .
@prefix dcat: <http://www.w3.org/ns/dcat#> .
@prefix xsd: <http://www.w3.org/2001/XMLSchema#> .

@prefix ids_da: <https://schema.industrialdataspace.org/dataAsset/> .
@prefix ids_rel: <https://schema.iais.fraunhofer.de/ids/helper/relation/> .
@prefix ids_doc: <https://schema.iais.fraunhofer.de/ids/helper/documentation/> .
@prefix ids_lang: <https://schema.industrialdataspace.org/language/> .
@prefix ids_trans: <https://schema.iais.fraunhofer.de/ids/helper/transformation/> .

# Classes
# -------

ids_da:Concept a owl:Class;
    rdfs:label "Concept"@en;
    rdfs:comment "References entry points to taxonomies of shared concepts (SKOS), e.g. Factory -> Automotive Factory."@en.

# Properties
# ----------

ids_da:coversCategory a owl:ObjectProperty;
    rdfs:subPropertyOf dcat:theme;
    rdfs:label "coversCategory"@en;
    ids_doc:labelPluralForm "coversCategories"@en;
    rdfs:domain ids_da:Concept;
    rdfs:range xsd:anyURI;
    rdfs:comment "Links to a taxonomy entry point that categorizes content-related coverage of the DataAsset."@en.

ids_da:keyword a owl:DatatypeProperty;
    rdfs:subPropertyOf dcat:theme;
    rdfs:label "keyword"@en;
    ids_doc:labelPluralForm "keywords"@en;
    rdfs:domain ids_da:Concept;
    rdfs:range xsd:anyURI;
    rdfs:comment "Links to an item in a flat list of controlled keywords that describe content-related coverage of the DataAsset."@en.
