@prefix owl: <http://www.w3.org/2002/07/owl#> .
@prefix rdfs: <http://www.w3.org/2000/01/rdf-schema#> .
@prefix xsd: <http://www.w3.org/2001/XMLSchema#> .
@prefix dct: <http://purl.org/dc/terms/> .
@prefix dcat: <http://www.w3.org/ns/dcat#> .

@prefix ids_da: <https://schema.industrialdataspace.org/dataAsset/> .
@prefix ids_content: <https://schema.industrialdataspace.org/content/Content> .
@prefix ids_base: <https://schema.industrialdataspace.org/base/> .
@prefix ids_rel: <https://schema.iais.fraunhofer.de/ids/helper/relation/> .
@prefix ids_conn: <https://schema.industrialdataspace.org/connector/> .

# Classes
# -------

ids_da:DataAsset rdfs:subClassOf ids_base:EntityWithLifecycle;
    rdfs:subClassOf ids_conn:ProvidedResource;
    rdfs:subClassOf dcat:Dataset;
    a owl:Class;
    rdfs:label "DataAsset"@en;
    rdfs:comment "Class describing data on the Industrial Dataspace. May be a data offering, data that is in the state of being transfered or an aggregation of multiple other dataassets."@en;
    ids_rel:validation [
        ids_rel:forProperty ids_da:coversTemporal;
        ids_rel:relationType ids_rel:OneToMany;
    ];
    ids_rel:validation [
        ids_rel:forProperty ids_da:coversSpatial;
        ids_rel:relationType ids_rel:OneToMany;
    ];
    ids_rel:validation [
        ids_rel:forProperty ids_da:coversCategory;
        ids_rel:relationType ids_rel:OneToMany;
    ].

# Properties
# ----------

ids_da:content a owl:ObjectProperty;
    rdfs:label "content"@en;
    rdfs:domain ids_da:DataAsset;
    rdfs:range ids_content:Content;
    rdfs:comment "Describes the content of the DataAsset."@en.

ids_da:commodity a owl:ObjectProperty;
    rdfs:label "commodity"@en;
    rdfs:domain ids_da:DataAsset;
    rdfs:range ids_da:Commodity;
    rdfs:comment "Describes the commodity facet of the DataAsset."@en.

ids_da:communication a owl:ObjectProperty;
    rdfs:label "communication"@en;
    rdfs:domain ids_da:DataAsset;
    rdfs:range ids_da:Communication;
    rdfs:comment "Describes the communication facet of the DataAsset, i.e. how it can be technically accessed."@en.

ids_da:concept a owl:ObjectProperty;
    rdfs:label "concept"@en;
    rdfs:domain ids_da:DataAsset;
    rdfs:range ids_da:Concept;
    rdfs:comment "Describes the concept facet of the DataAsset, i.e. how it can be categorized."@en.

ids_da:contract a owl:ObjectProperty;
    rdfs:label "contract"@en;
    rdfs:domain ids_da:DataAsset;
    rdfs:range ids_da:Contract;
    rdfs:comment "Describes the contract facet of the DataAsset, e.g., terms of use, service level agreements,..."@en.

ids_da:context a owl:ObjectProperty;
    rdfs:label "context"@en;
    rdfs:domain ids_da:DataAsset;
    rdfs:range ids_da:Context;
    rdfs:comment "Describes the context facet of the DataAsset, i.e., its relation to the world in terms of, e.g, spatial and timely dimensions."@en.

ids_da:version rdfs:subPropertyOf dct:hasVersion;
    a owl:DatatypeProperty;
    rdfs:label "version"@en;
    rdfs:domain ids_da:DataAsset;
    rdfs:range xsd:string;
    rdfs:comment "Version identifier of the InfrastructureComponent."@en.