@prefix owl: <http://www.w3.org/2002/07/owl#> .
@prefix rdfs: <http://www.w3.org/2000/01/rdf-schema#> .
@prefix dct: <http://purl.org/dc/terms/> .
@prefix xsd: <http://www.w3.org/2001/XMLSchema#> .
@prefix odrl: <http://www.w3.org/ns/odrl/2/> .
@prefix ids: <https://w3id.org/ids/core/> .
@prefix idsm: <https://w3id.org/ids/metamodel/> .

# Classes
# -------

ids:CommodizationModel
    a owl:Class ;
    rdfs:label "Commodization model"@en;
    rdfs:comment "Overall commodization model composed of options."@en ;
    idsm:abstract true .

ids:CommodizationOption
    a owl:Class ;
    rdfs:label "Commodization option"@en;
    rdfs:comment "Option of turning a Resource or Service into a product."@en ;
    idsm:abstract true .

# Distinction according to fee-based/chargeable use
#
ids:FreeUse # Pattern: Free
    a owl:Class ;
    rdfs:subClassOf ids:CommodizationOption ;
    rdfs:label "Free use"@en;
    rdfs:comment "The product is free of charge, its usage is optionally restricted by non-financial constraints (licence etc.)."@en .
    
ids:ChargeableUse
    a owl:Class ;
    rdfs:subClassOf ids:CommodizationOption ;
    rdfs:label "Chargeable use"@en;
    rdfs:comment "The product is subject to a fee-based use."@en ;
    idsm:abstract true ;
    owl:disjointWith ids:FreeUse .

# Distinction according to type of charged product
#
ids:ConsumptionBasedPricing # Pattern: Pay-per-Use / Pay on demand etc.
    a owl:Class ;
    rdfs:subClassOf ids:ChargeableUse ;
    rdfs:label "Consumption-based pricing"@en;
    rdfs:comment "The product is charged based on the actual consumption."@en ;
    idsm:abstract true .

ids:QuantityBasedPricing
    a owl:Class ;
    rdfs:subClassOf ids:ConsumptionBasedPricing ;
    rdfs:label "Quantity-based pricing"@en;
    rdfs:comment "The product is charged based on a quantifiable amount (i.e. data volume or number of API calls)."@en .

ids:FeatureBasedPricing
    a owl:Class ;
    rdfs:subClassOf ids:ConsumptionBasedPricing ;
    rdfs:label "Feature-based pricing"@en;
    rdfs:comment "The product is charged based on a selection of features (i.e. map overlays, service set etc.)"@en .
    
ids:FlatratePricing # Pattern: Flat Rate / Subscription etc.
    a owl:Class ;
    rdfs:subClassOf ids:ChargeableUse ;
    rdfs:label "Flatrate pricing"@en;
    rdfs:comment "The product is charged on subscription base independently of the actual consumption."@en ;
    owl:disjointWith ids:ConsumptionBasedPricing .
    
ids:FreemiumModel # Pattern: Freemium
    a owl:Class ;
    rdfs:subClassOf ids:CommodizationModel ;
    rdfs:label "Freemium model"@en ;
    rdfs:comment "Commodization model offering free and advanced commercial use."@en ;
    rdfs:subClassOf [
        a owl:Restriction ;
        owl:onProperty ids:commodizationOption ;
        owl:someValuesFrom ids:FreeUse  
    ] ;
    rdfs:subClassOf [
        a owl:Restriction ;
        owl:onProperty ids:commodizationOption ;
        owl:someValuesFrom ids:ChargeableUse # Consumption-based or Flatrate
    ] .
    
# Properties
# ----------

ids:commodizationOption a owl:CommodizationOption;
    rdfs:label "commodization option"@en;
    rdfs:domain ids:CommodizationModel;
    rdfs:range ids:CommodizationOption;
    rdfs:comment "Commodization option supplied by the model."@en.




        
    


ids:UsagePolicy rdfs:subClassOf odrl:Policy;
    rdfs:label "Usage policy"@en;
    rdfs:comment "Set of rules specified by the Data Sovereign restricting usage of its data; covers aspects like time-to-live or forwarding conditions (e.g., anonymization or scope of usage); transmitted along with the respective data, and enforced while residing on the Connector of the Data Consumer"@en .
    
