@prefix owl: <http://www.w3.org/2002/07/owl#> .
@prefix rdf: <http://www.w3.org/1999/02/22-rdf-syntax-ns#> .
@prefix rdfs: <http://www.w3.org/2000/01/rdf-schema#> .
@prefix xsd: <http://www.w3.org/2001/XMLSchema#> .
@prefix dct: <http://purl.org/dc/terms/> .
@prefix ids: <https://w3id.org/ids/core/> .
@prefix idsm: <https://w3id.org/ids/metamodel/> .

# Classes
# -------

ids:ProtocolBinding a owl:Class;
    idsm:abstract true;
    rdfs:label "ProtocolBinding"@en;
    rdfs:comment "Mapping of abstract operation signatures onto the concrete structures (e.g., HTTP headers or query parameters)."@en.

ids:HttpProtocolBinding a owl:Class;
    rdfs:subClassOf ids:ProtocolBinding;
    rdfs:label "HttpProtocolBinding"@en;
    rdfs:comment "Class of mapping of abstract operation signatures to the HTTP protocol."@en.

ids:MqttProtocolBinding a owl:Class;
    rdfs:subClassOf ids:ProtocolBinding;
    rdfs:label "MqttProtocolBinding"@en;
    rdfs:comment "Class of mapping of abstract operation signatures to the MQTT protocol."@en.

ids:ApiDocument a owl:Class;
    rdfs:label "ApiDocument"@en;
    rdfs:comment "Class of documents, fully and consistently describing an API, e.g., according to the OpenAPI specification."@en.

ids:Endpoint a owl:Class;
    rdfs:label "Endpoint"@en;
    rdfs:comment "Class of invokable network Endpoints that return a DataAsset."@en.

# General Properties
# ------------------

ids:apiDocument a owl:ObjectProperty;
    rdfs:label "apiDocument"@en;
    rdfs:domain ids:ProtocolBinding;
    rdfs:range ids:ApiDocument;
    rdfs:comment "Document describing the API of the binding."@en.

ids:apiDocumentReference a owl:DatatypeProperty;
    rdfs:label "apiDocumentReference"@en;
    rdfs:domain ids:ProtocolBinding;
    rdfs:range xsd:string;
    rdfs:comment "References a structure inside the ApiDocument's content, e.g., a JSON path for OpenAPI documents."@en.

ids:apiDocumentType a owl:ObjectProperty;
    rdfs:label "apiDocumentType"@en;
    rdfs:domain ids:ApiDocument;
    rdfs:range ids:ApiDocumentType;
    rdfs:comment "Type of the ApiDocument."@en.

ids:documentContent a owl:DatatypeProperty;
    rdfs:label "content"@en;
    rdfs:domain ids:ApiDocument;
    rdfs:range xsd:string;
    rdfs:comment "Textual representation of an API description, e.g., the OpenAPI JSON structure."@en.

ids:endpoint a owl:ObjectProperty;
    rdfs:label "endpoint"@en;
    rdfs:domain ids:ProtocolBinding;
    rdfs:range ids:Endpoint;
    rdfs:comment "Reference to be invoked in order to retrieve a DataAsset."@en.

# Properties of Endpoint
# ----------------------

ids:url a owl:DatatypeProperty;
    rdfs:label "url"@en;
    rdfs:domain ids:Endpoint;
    rdfs:range xsd:anyURI;
    rdfs:comment "URI that returns a certain representation of a DataAsset."@en.

# Properties
# ----------

ids:topic a owl:DatatypeProperty;
    rdfs:label "topic"@en;
    rdfs:domain ids:MqttProtocolBinding;
    rdfs:range xsd:string;
    rdfs:comment "Defines a topic that is used for message exchange."@en.

ids:messageBroker a owl:DatatypeProperty;
    rdfs:label "messageBroker"@en;
    rdfs:domain ids:MqttProtocolBinding;
    rdfs:range xsd:anyURI;
    rdfs:comment "Location of the MQTT message broker."@en.


