@prefix dct: <http://purl.org/dc/terms/> .
@prefix dcmitype: <http://purl.org/dc/dcmitype/> .
@prefix ids: <https://w3id.org/ids/core/> .
@prefix idsm: <https://w3id.org/ids/metamodel/> .
@prefix owl: <http://www.w3.org/2002/07/owl#> .
@prefix rdf: <http://www.w3.org/1999/02/22-rdf-syntax-ns#> .
@prefix rdfs: <http://www.w3.org/2000/01/rdf-schema#> .
@prefix skos: <http://www.w3.org/2004/02/skos/core#> .
@prefix xsd: <http://www.w3.org/2001/XMLSchema#> .

# Classes
# -------

ids:ContentType
    rdf:type owl:Class ;
    idsm:abstract true ;
    rdfs:label "Content type"@en ;    
    rdfs:comment "Nature of a Digital Content providing hints on its usage, e.g. navigating a Structure or accessing a List by an index." ;
    # discuss: rdfs:subClassOf dct:DCMIType or ..?    
    rdfs:seeAlso <http://www.ontodm.com/doku.php?id=ontodt> ;
    rdfs:seeAlso <https://schema.org/DataType> ;
    rdfs:seeAlso <https://schema.org/additionalType> .

# Abstract content types
# ----------------------

# ids:Named - via dct.Identifier?

ids:Ordered
    rdfs:subClassOf ids:ContentType ;
    owl:equivalentClass
    [
      rdf:type          owl:Restriction ;
      owl:onProperty    ids:ordered ;
      owl:hasValue      "true"^^xsd:boolean 
    ];
    rdfs:label "Ordered content"@en ;
    rdfs:comment "Type of Digital Content ordered in a particular way. Serves as rdfs:domain of ordering-related properties."@en .

#ids:Homogenous
#    rdfs:subClassOf ids:ContentType ;
#    owl:equivalentClass
#    [
#      rdf:type          owl:Restriction ;
#      owl:onProperty    ids:homogenous ;
#      owl:hasValue      "true"^^xsd:boolean 
#    ];
#    rdfs:label "Homogenous content"@en ;
#    rdfs:comment "Type of Digital Content that is homogenous (with regards to Data Type and Serialization) thus allows for a uniform processing."@en .

# Abstract data types
# -------------------

ids:Opaque a owl:Class;
    rdfs:subClassOf ids:ContentType ;
    owl:disjointWith ids:Structure ;
    rdfs:label "Opaque"@en ;
    rdfs:comment "Opaque type of Resource that is not further specified."@en .
    
ids:Structure a owl:Class;
    rdfs:subClassOf ids:ContentType ;
    owl:disjointWith ids:RawType ;
    rdfs:label "Structure"@en ;
    skos:altLabel "Record"@en ;
    skos:altLabel "Struct"@en ;
    rdfs:comment "Custom or generic structured data type, i.e. arrangement of data fields (possibly named, ordered, strongly typed etc.)."@en ;
    rdfs:seeAlso <https://schema.org/StructuredValue> .
    
ids:Value a owl:Class;
    rdfs:subClassOf ids:ContentType ;
    owl:disjointWith ids:Opaque, ids:Structure ;
    rdfs:label "Value"@en ;
    rdfs:comment "Terminal node, from the modeling perspective an atomic, possibly typed value."@en .
    
ids:Collection a owl:Class;
    rdfs:subClassOf ids:Structure ;
    idsm:abstract true ;
    rdfs:label "Collection"@en ;
    rdfs:comment "Group of entities supporting particular access operations based on the concrete subclass."@en ;
    rdfs:seeAlso <https://docs.oracle.com/javase/8/docs/technotes/guides/collections/overview.html> .
    
ids:Map a owl:Class;
    rdfs:subClassOf ids:Collection ;
    rdfs:label "Map"@en ;
    rdfs:comment "Collection of Resources allowing for a key based access."@en ;
    rdfs:seeAlso <https://docs.oracle.com/javase/8/docs/api/java/util/Map.html> .

ids:List a owl:Class;
    rdfs:subClassOf ids:Ordered, ids:Collection ;
    rdfs:label "List"@en ;
    rdfs:comment "Ordered Collection of Resources allowing for an index-based access."@en ;
    rdfs:seeAlso <https://docs.oracle.com/javase/8/docs/api/java/util/List.html> .

ids:Application a owl:Class ;
    rdfs:subClassOf ids:ContentType ;
    rdfs:label "Application"@en ;
    rdfs:comment "IDS Application."@en .

ids:SortOrder a owl:Class ;
    rdfs:label "Sort order"@en ;    
    rdfs:comment "Sort order of entries within an ordered Collection."@en .
    
# Properties
# ----------

ids:ordered
    a owl:DatatypeProperty ;
    rdfs:label "ordered"@en;
    rdfs:domain ids:ContentType ;
    rdfs:range xsd:boolean ;
    rdfs:comment "Property indicating whether this type of Content supports ordering in a particular way (natural and user-driven ordering)."@en .

# Renamed from orderPolicy
ids:sortOrder a owl:ObjectProperty;
    rdfs:label "sort order"@en;
    rdfs:domain ids:Ordered;
    rdfs:range ids:SortOrder;
    rdfs:comment "Indicates the sort order of an ordered Collection."@en.

# clarify:
#
#ids:homogenous
#    a owl:DatatypeProperty ;
#    rdfs:label "homogenous"@en ;
#    rdfs:domain ids:ContentType ;
#    rdfs:range xsd:boolean ;
#    rdfs:comment "Flag indicating whether the Content parts are homogenous."@en .
#
#ids:orderBy a owl:ObjectProperty;
#    rdfs:label "orderBy"@en;
#    rdfs:domain ids:Ordered;
#    TODO, discuss: what is the appropriate range here / how do we link columns etc. -> Content /rdfs:Resource?
#    rdfs:range ids:Content;
#    rdfs:comment "Content (field) defining the current sort order of an ordered Content."@en.
#
#ids:key a owl:ObjectProperty;
#    rdfs:label "key"@en;
#    rdfs:domain ids:MapKind;
#    rdfs:range ids:Kind;
#    rdfs:comment "Describes the type of the key that indexes a Map."@en.
#
#ids:values a owl:ObjectProperty;
#    rdfs:label "values"@en;
#    rdfs:domain ids:MapKind;
#    rdfs:range ids:Kind;
#    rdfs:comment "Describes the type of the indexed values of a Map."@en.

## Instances
## ---------

#ids:hash a ids:ContentType;
#    rdfs:comment "hash";
#    dct:identifier "HASH".
#
#ids:date a ids:ContentType;
#    rdfs:comment "date";
#    dct:identifier "DATE";
#    skos:narrower ids:startDate;
#    skos:narrower ids:endDate.
#
#ids:startDate a ids:ContentType;
#    rdfs:comment "start date";
#    dct:identifier "START_DATE";
#    skos:broader ids:date.
#
#ids:endDate a ids:ContentType;
#    rdfs:comment "end date";
#    dct:identifier "END_DATE" ;
#    skos:broader ids:date.
#
#ids:textual a ids:ContentType;
#    rdfs:comment "textual";
#    dct:identifier "TEXTUAL";
#    skos:narrower ids:freetext.
#
#ids:binary a ids:ContentType;
#    rdfs:comment "binary";
#    dct:identifier "BINARY".
#
#ids:image a ids:ContentType;
#    rdfs:comment "image";
#    dct:identifier "IMAGE".
#
#ids:identifier a ids:ContentType;
#    rdfs:comment "identifier";
#    dct:identifier "IDENTIFIER".
#
#ids:weatherStationId a ids:ContentType;
#    rdfs:comment "weatherStationId";
#    dct:identifier "WEATHER_STATION_ID".
#
#ids:freetext a ids:ContentType;
#    rdfs:comment "freetext";
#    dct:identifier "FREETEXT";
#    skos:broader ids:textual.
#
#ids:sensor a ids:ContentType;
#    rdfs:comment "sensor measurement";
#    dct:identifier "SENSOR_MEASUREMENT".
#
# add "IDS Transfer Metadata" as content type
