@prefix owl: <http://www.w3.org/2002/07/owl#> .
@prefix rdfs: <http://www.w3.org/2000/01/rdf-schema#> .
@prefix xsd: <http://www.w3.org/2001/XMLSchema#> .
@prefix credential: <http://www.daml.org/services/owl-s/security/credential.owl#> .
@prefix dct: <http://purl.org/dc/terms/> .
@prefix ids: <https://w3id.org/ids/core/> .
@prefix idsm: <https://w3id.org/ids/metamodel/> .

# Classes
# -------

ids:DataTransfer
	a owl:Class;
    rdfs:subClassOf ids:Message;
	rdfs:label "DataTransfer"@en;
	rdfs:comment "The class of resources that describe a data transfer on the IDS."@en;
    idsm:validation [
        idsm:forProperty ids:transferCreatedAt;
        idsm:constraint idsm:NotNull;
    ].

ids:PublicKey a owl:Class;
	rdfs:label "PublicKey"@en;
	rdfs:comment "The class of resources that describe a data transfer on the IDS."@en.

# Properties of DataTransfer
# --------------------------

ids:transferContract
	a owl:ObjectProperty;
	rdfs:label "transferContract"@en;
	rdfs:domain ids:DataTransfer;
	rdfs:range ids:Contract;
	rdfs:comment "The contract which is (or will be) the legal basis of the data transfer."@en.

ids:payloadSignature
	a owl:DatatypeProperty;
	rdfs:label "payload signature"@en;
	rdfs:domain ids:DataTransfer;
	rdfs:range xsd:base64Binary;
	rdfs:comment "Digital signature of the data payload associated to this DataTransfer instance."@en.

ids:senderPublicKey
	a owl:ObjectProperty;
	rdfs:label "sender public key"@en;
	rdfs:domain ids:DataTransfer;
	rdfs:range ids:PublicKey;
	rdfs:comment "The public key of the sending connector."@en.

# Properties of PublicKey
# -----------------------

ids:keyPairAlgorithm a owl:ObjectProperty;
    rdfs:label "keyPairAlgorithm"@en;
    rdfs:domain ids:PublicKey;
    rdfs:range ids:KeyPairAlgorithm;
    rdfs:comment "Algorithm used to generate the public key."@en.

ids:keyValue a owl:DatatypeProperty;
    rdfs:label "keyValue"@en;
    rdfs:domain ids:PublicKey;
    rdfs:range xsd:base64Binary;
    rdfs:comment "Encoded value of the key."@en.

# todo: we also need to add a property that holds the instances of the operation parameters


