@prefix owl: <http://www.w3.org/2002/07/owl#> .
@prefix rdf: <http://www.w3.org/1999/02/22-rdf-syntax-ns#> .
@prefix rdfs: <http://www.w3.org/2000/01/rdf-schema#> .
@prefix xsd: <http://www.w3.org/2001/XMLSchema#> .
@prefix dct: <http://purl.org/dc/terms/> .
@prefix ids: <https://w3id.org/ids/core/> .
@prefix idsm: <https://w3id.org/ids/metamodel/> .

# Classes
# -------

ids:Endpoint a owl:Class ;
	idsm:abstract true;
	rdfs:label "Endpoint"@en ;
    rdfs:comment "Data exchange point for publication (Data Source) and/or consumption (Data Sink) of Communicable objects."@en .

ids:DataSink
	rdfs:subClassOf ids:Endpoint ;
	rdfs:label "Data Sink"@en ;
    rdfs:comment "Endpoint consuming data supplied by a Data Provider."@en .

ids:DataSource
	rdfs:subClassOf ids:Endpoint ;
	rdfs:label "Data Source"@en ;
    rdfs:comment "Endpoint exposing data for being retrieved or subscribed to by a Data Consumer."@en .

ids:HttpEndpoint
    a owl:Class ;
	rdfs:label "HTTP endpoint"@en ;
    rdfs:comment "Endpoint operated via HTTP accessible at a URL."@en .


# Properties of Endpoint
# ----------------------

ids:url a owl:DatatypeProperty;
    rdfs:label "url"@en;
    rdfs:domain ids:HttpEndpoint;
    rdfs:range xsd:anyURI;
    rdfs:comment "url exposing an instance or the access service of a Resource."@en.

ids:resourceInstance a owl:ObjectProperty;
    rdfs:label "resource instance"@en;
    rdfs:domain ids:HttpEndpoint;
    rdfs:range ids:Artifact;
    rdfs:comment "Artifact exposed by the HTTP Endpoint."@en.

ids:resourceService a owl:ObjectProperty;
    rdfs:label "resource service"@en;
    rdfs:domain ids:HttpEndpoint;
    rdfs:range ids:ResourceService;
    rdfs:comment "Resource service exposed by the HTTP Endpoint."@en.
    
