@prefix owl: <http://www.w3.org/2002/07/owl#> .
@prefix rdf: <http://www.w3.org/1999/02/22-rdf-syntax-ns#> .
@prefix rdfs: <http://www.w3.org/2000/01/rdf-schema#> .
@prefix xsd: <http://www.w3.org/2001/XMLSchema#> .
@prefix dct: <http://purl.org/dc/terms/> .
@prefix ids: <https://w3id.org/ids/core/> .
@prefix idsm: <https://w3id.org/ids/metamodel/> .

# Classes
# -------

ids:Endpoint a owl:Class ;
	idsm:abstract true;
	rdfs:label "Endpoint"@en ;
    rdfs:comment "Access point of data exchange and service interaction."@en .

ids:DataSink
    idsm:abstract true ;
	rdfs:subClassOf ids:Endpoint ;
	rdfs:label "Data Sink"@en ;
    rdfs:comment "Endpoint consuming digital content supplied by a Data Provider."@en .

ids:DataSource
    idsm:abstract true ;
	rdfs:subClassOf ids:Endpoint ;
	rdfs:label "Data Source"@en ;
    rdfs:comment "Endpoint providing digital content for being retrieved or subscribed to by a Data Consumer."@en .

ids:HttpEndpoint a owl:Class ;
    rdfs:subClassOf ids:Endpoint ;
	rdfs:label "HTTP endpoint"@en ;
    rdfs:comment "Endpoint exposed via the Hypertext Transfer Protocol."@en .

ids:MqttEndpoint a owl:Class ;
    rdfs:subClassOf ids:Endpoint ;
	rdfs:label "MQTT endpoint"@en ;
    rdfs:comment "Endpoint exposed via the Message Queuing Telemetry Transport protocol."@en .

# Properties of Endpoint
# ----------------------

ids:endpointHost
    a owl:ObjectProperty;
    rdfs:label "endpoint host"@en;
    rdfs:domain ids:Endpoint;
    rdfs:range ids:Host;
    rdfs:comment "Network host that exposes resource content and Connector services via this endpoint."@en ;
    idsm:referenceByUrl true .

ids:endpointContent
    a owl:ObjectProperty;
    rdfs:label "endpoint content"@en;
    rdfs:domain ids:Endpoint;
    rdfs:range ids:Instance;
    rdfs:comment "Content instance mediated via this individual endpoint (1:1 mapping)."@en ;
    idsm:referenceByUrl true .
    
# Properties of HttpEndpoint
# --------------------------
# apply to IDSCP as well

ids:path
    a owl:DatatypeProperty;
    rdfs:label "path"@en;
    rdfs:domain ids:HttpEndpoint;
    rdfs:range xsd:string;
    rdfs:comment "Absolute path at which the content is published by the related host."@en.

# Properties of MqttEndpoint
# --------------------------

ids:topic
    a owl:DatatypeProperty;
    rdfs:label "topic"@en;
    rdfs:domain ids:MqttEndpoint;
    rdfs:range xsd:string;
    rdfs:comment "Topic used for bi-directional MQTT communication via this endpoint."@en.

ids:inboundTopic
    a owl:DatatypeProperty;
    rdfs:label "inbound topic"@en;
    rdfs:domain ids:MqttEndpoint;
    rdfs:range xsd:string;
    rdfs:comment "Topic used for inbound MQTT communication via this endpoint, i.e. input messages and faults only."@en.

ids:outboundTopic
    a owl:DatatypeProperty;
    rdfs:label "outbound topic"@en;
    rdfs:domain ids:MqttEndpoint;
    rdfs:range xsd:string;
    rdfs:comment "Topic used for outbound MQTT communication via this endpoint, i.e. output messages and faults only."@en.
