@prefix owl: <http://www.w3.org/2002/07/owl#> .
@prefix rdf:   <http://www.w3.org/1999/02/22-rdf-syntax-ns#> .
@prefix rdfs: <http://www.w3.org/2000/01/rdf-schema#> .
@prefix xsd: <http://www.w3.org/2001/XMLSchema#> .
@prefix dct: <http://purl.org/dc/terms/> .
@prefix ids: <https://w3id.org/ids/core/> .
@prefix idsm: <https://w3id.org/ids/metamodel/> .

# Classes
# -------

ids:Message a owl:Class;
    rdfs:label "Message"@en ;
    idsm:abstract true;
	rdfs:comment "Metadata describing payload exchanged by interacting Connectors."@en ;
    idsm:validation [
        idsm:forProperty ids:modelVersion;
        idsm:constraint idsm:NotNull;
    ];
    idsm:validation [
        idsm:forProperty ids:issued;
        idsm:constraint idsm:NotNull;
    ];
    idsm:validation [
        idsm:forProperty ids:issuingConnector;
        idsm:constraint idsm:NotNull;
    ].
    # FIPA ACL Message Structure Specification, http://www.fipa.org/specs/fipa00061/index.html

# Properties
# ----------

ids:modelVersion
    a owl:DatatypeProperty;
    rdfs:label "model version"@en;
    rdfs:domain ids:Message;
    rdfs:range xsd:string;
    rdfs:comment "Version of the Information Model against which the Message should be interpreted."@en.

ids:issued
    rdfs:subPropertyOf dct:issued;
    a owl:DatatypeProperty;
    rdfs:label "issued"@en;
    rdfs:domain ids:Message;
    rdfs:range xsd:dateTime;
    rdfs:comment "Date of issuing the Message."@en.

ids:correlationMessage
	a owl:ObjectProperty;
	rdfs:label "consumer connector"@en;
	rdfs:domain ids:Message;
	rdfs:range ids:MessageIdentifier; # implies reference to a corelated Message
	rdfs:comment "Correlated message, e.g. a response to a previous request."@en.

ids:issuingConnector
	a owl:DatatypeProperty;
	rdfs:label "provider connector"@en;
	rdfs:domain ids:Message;
	rdfs:range ids:ConnectorIdentifier;# implies reference to Data Provider
	rdfs:comment "The Connector which is the origin of the message."@en.

ids:consumerConnector
	a owl:ObjectProperty;
	rdfs:label "consumer connector"@en;
	rdfs:domain ids:Message;
	rdfs:range ids:ConnectorIdentifier;# implies reference to Data Consumer
	rdfs:comment "The Connector which is the recipient of the message."@en.

ids:senderAgent
	a owl:DatatypeProperty;
	rdfs:label "sender agent"@en;
	rdfs:domain ids:DataTransfer;
	rdfs:range ids:AgentIdentifier;#  terminal origin e.g. the Data Sovereign
	rdfs:comment "The Agent which initiated the Message."@en.

ids:recipientAgent 
	a owl:DatatypeProperty;
	rdfs:label "recipient agent"@en;
	rdfs:domain ids:Message;
	rdfs:range ids:AgentIdentifier;# terminal addressee e.g. the Data User
	rdfs:comment "The Agent for which the Mesaage is intended."@en.

ids:authorizationToken
	a owl:ObjectProperty;
	rdfs:label "authorization token"@en;
	rdfs:domain ids:Message;
	rdfs:range ids:AuthorizationToken;
	rdfs:comment "An authorization token like JSON Web Token."@en.

## .. check:
  
ids:BrokerMessage rdfs:subClassOf ids:Message;
    a owl:Class;
    rdfs:label "BrokerMessage"@en ;
    idsm:abstract true;
    rdfs:comment "The class of all messages to interact with a Broker.";
    idsm:validation [
        idsm:forProperty ids:messageContent;
        idsm:constraint idsm:NotNull;
    ].

ids:BrokerDataMessage rdfs:subClassOf ids:BrokerMessage;
    a owl:Class;
    idsm:abstract true;
    rdfs:label "BrokerDataMessage"@en ;
    rdfs:comment "The class of all messages intended for data transfer to/from a Broker.".

ids:BrokerQueryMessage rdfs:subClassOf ids:BrokerMessage;
    a owl:Class;
    idsm:abstract true;
    rdfs:label "BrokerQueryMessage"@en ;
    rdfs:comment "The class of all messages that query the broker for data.".

ids:BrokerRequestMessage rdfs:subClassOf ids:BrokerMessage;
    a owl:Class;
    idsm:abstract true;
    rdfs:label "BrokerRequestMessage"@en ;
    rdfs:comment "The class of all messages that represent requests to a Broker.";
    idsm:validation [
        idsm:forProperty ids:coveredEntity;
        idsm:constraint idsm:NotNull;
    ].

ids:BrokerResponseMessage rdfs:subClassOf ids:BrokerMessage;
    a owl:Class;
    idsm:abstract true;
    rdfs:label "BrokerResponseMessage"@en ;
    rdfs:comment "The class of all messages that represent responses of a Broker.";
    idsm:validation [
        idsm:forProperty ids:correlationId;
        idsm:constraint idsm:NotNull;
    ].

ids:BrokerDataRequest rdfs:subClassOf ids:BrokerDataMessage, ids:BrokerRequestMessage;
    a owl:Class;
    rdfs:label "BrokerDataRequest"@en ;
    rdfs:comment "The class of all messages that represent data requests to a Broker.";
    idsm:validation [
        idsm:forProperty ids:dataRequestAction;
        idsm:constraint idsm:NotNull;
    ].

ids:BrokerDataResponse rdfs:subClassOf ids:BrokerDataMessage, ids:BrokerResponseMessage;
    a owl:Class;
    rdfs:label "BrokerDataResponse"@en ;
    rdfs:comment "The class of all messages that represent data responses of a Broker.".

ids:BrokerQueryRequest rdfs:subClassOf ids:BrokerRequestMessage, ids:BrokerQueryMessage;
    a owl:Class;
    rdfs:label "BrokerQueryRequest"@en ;
    rdfs:comment "The class of all messages that represent query requests to a Broker.";
    idsm:validation [
        idsm:forProperty ids:queryRequestAction;
        idsm:constraint idsm:NotNull;
    ];
    idsm:validation [
        idsm:forProperty ids:queryScope;
        idsm:constraint idsm:NotNull;
    ].

ids:BrokerQueryResponse rdfs:subClassOf ids:BrokerQueryMessage, ids:BrokerResponseMessage;
    a owl:Class;
    rdfs:label "BrokerQueryResponse"@en ;
    rdfs:comment "The class of all messages that represent a Broker's response to a query.".

# Classes with a fixed set of instances
# -------------------------------------

ids:BrokerDataRequestAction a owl:Class;
    rdfs:label "BrokerDataRequestAction"@en ;
    rdfs:comment "The class of all actions that can be issued to a broker in a data request message.".

ids:BrokerDataRegisterAction a ids:BrokerDataRequestAction;
    idsm:constantIdentifier "REGISTER"@en.

ids:BrokerDataUpdateAction a ids:BrokerDataRequestAction;
    idsm:constantIdentifier "UPDATE"@en.

ids:BrokerDataPassivateAction a ids:BrokerDataRequestAction;
    idsm:constantIdentifier "PASSIVATE"@en.

ids:BrokerDataActivateAction a ids:BrokerDataRequestAction;
    idsm:constantIdentifier "ACTIVATE"@en.

ids:BrokerDataRemoveAction a ids:BrokerDataRequestAction;
    idsm:constantIdentifier "REMOVE"@en.

ids:BrokerQueryRequestAction a owl:Class;
    rdfs:label "BrokerQueryRequestAction"@en ;
    rdfs:comment "The class of all actions that can be issued to a broker in a query message.".

ids:BrokerQueryRequestGetAction a ids:BrokerQueryRequestAction;
    idsm:constantIdentifier "GET"@en.

ids:BrokerQueryRequestListAction a ids:BrokerQueryRequestAction;
    idsm:constantIdentifier "LIST"@en.

ids:BrokerQueryRequestQueryAction a ids:BrokerQueryRequestAction;
    idsm:constantIdentifier "QUERY"@en.

ids:BrokerQueryMessageScope a owl:Class;
    rdfs:label "BrokerQueryMessageScope"@en ;
    rdfs:comment "The class of scopes that filter datasets by their states when queried.".

ids:BrokerQueryMessageScopeAll a ids:BrokerQueryMessageScope;
    idsm:constantIdentifier "ALL"@en.

ids:BrokerQueryMessageScopeActive a ids:BrokerQueryMessageScope;
    idsm:constantIdentifier "ACTIVE"@en.

ids:BrokerQueryMessageScopeAccess a ids:BrokerQueryMessageScope;
    idsm:constantIdentifier "ACCESS"@en.

ids:EntityCoveredByDataRequest a owl:Class;
    rdfs:label "EntityCoveredByDataRequest"@en ;
    rdfs:comment "The class of IDS entities that are described in a BrokerDataRequest message.".

ids:CoveredParticipant a ids:EntityCoveredByDataRequest;
    idsm:constantIdentifier "PARTICIPANT"@en.

ids:CoveredConnector a ids:EntityCoveredByDataRequest;
    idsm:constantIdentifier "CONNECTOR"@en.

ids:CoveredDataEndpoint a ids:EntityCoveredByDataRequest;
    idsm:constantIdentifier "DATA_ENDPOINT"@en.

# Properties
# ----------

ids:dataRequestAction a owl:ObjectProperty;
    rdfs:label "dataRequestAction"@en;
    rdfs:domain ids:BrokerDataRequest;
    rdfs:range ids:BrokerDataRequestAction;
    rdfs:comment "The action that should be performed with the message's content at the Broker."@en.

ids:queryRequestAction a owl:ObjectProperty;
    rdfs:label "queryRequestAction"@en;
    rdfs:domain ids:BrokerQueryRequest;
    rdfs:range ids:BrokerQueryRequestAction;
    rdfs:comment "The action that should be performed by the query."@en.

ids:coveredEntity a owl:ObjectProperty;
    rdfs:label "coveredEntity"@en;
    rdfs:domain ids:BrokerRequestMessage;
    rdfs:range ids:EntityCoveredByDataRequest;
    rdfs:comment "The IDS entity covered in the data request."@en.

ids:messageContent a owl:DatatypeProperty;
    rdfs:label "messageContent"@en;
    rdfs:domain ids:BrokerMessage;
    rdfs:range xsd:string;
    rdfs:comment "The message's content, e.g., a query."@en.

ids:correlationId a owl:DatatypeProperty;
    rdfs:label "correlationId"@en;
    rdfs:domain ids:BrokerResponseMessage;
    rdfs:range xsd:anyURI;
    rdfs:comment "The unique ID of the source request which is referred to by a response message."@en.

ids:queryScope a owl:ObjectProperty;
    rdfs:label "queryScope"@en;
    rdfs:domain ids:BrokerQueryMessage;
    rdfs:range ids:BrokerQueryMessageScope;
    rdfs:comment "The scope of a query defined in a query message."@en.
