@prefix rdf:   <http://www.w3.org/1999/02/22-rdf-syntax-ns#> .
@prefix owl: <http://www.w3.org/2002/07/owl#> .
@prefix rdfs: <http://www.w3.org/2000/01/rdf-schema#> .
@prefix xsd: <http://www.w3.org/2001/XMLSchema#> .
@prefix dcat: <http://www.w3.org/ns/dcat#> .
@prefix ids: <https://w3id.org/idsa/core/> .
@prefix idsm: <https://w3id.org/idsa/metamodel/> .

# Classes
# -------

ids:Catalog
    a owl:Class;
    rdfs:subClassOf dcat:Catalog;
    idsm:abstract true;
    rdfs:label "Catalog"@en ;
    rdfs:comment "Class that represents (distributable) Catalogs."@en ;
    .

ids:ResourceCatalog
    a owl:Class;
    rdfs:subClassOf ids:Catalog;
    rdfs:label "Resource Catalog"@en ;
    rdfs:comment "Class that aggregates Resources which, as a whole, form a (distributable) Catalog."@en ;
    idsm:validation [
        idsm:forProperty ids:requestedResource;
        idsm:relationType idsm:OneToMany;
    ];
    idsm:validation [
        idsm:forProperty ids:offeredResource;
        idsm:relationType idsm:OneToMany;
    ];
.

ids:ParticipantCatalog
    a owl:Class;
    rdfs:subClassOf ids:Catalog;
    rdfs:label "Participant Catalog"@en ;
    rdfs:comment "Class that aggregates Participants, as a whole, from a (distributable) Catalog."@en ;
    idsm:validation [
        idsm:forProperty ids:member;
        idsm:relationType idsm:OneToMany;
    ];
.

ids:ConnectorCatalog
    a owl:Class;
    rdfs:subClassOf ids:Catalog;
    rdfs:label "Connector Catalog"@en ;
    rdfs:comment "Class that aggregates Connectors, as a whole, from a (distributable) Catalog."@en ;
    idsm:validation [
        idsm:forProperty ids:listedConnector;
        idsm:relationType idsm:OneToMany;
    ];
.

ids:BrokerCatalog
    a owl:Class;
    rdfs:subClassOf ids:ConnectorCatalog;
    rdfs:label "Broker Catalog"@en ;
    rdfs:comment "Class that aggregates Brokers, as a whole, from a (distributable) Catalog."@en ;
.

ids:AppStoreCatalog
    a owl:Class;
    rdfs:subClassOf ids:ConnectorCatalog;
    rdfs:label "AppStore Catalog"@en ;
    rdfs:comment "Class that aggregates AppStores , as a whole, from a (distributable) Catalog."@en ;
.

# TODO: Align with ResourceCatalog
ids:AppResourceCatalog
    a owl:Class;
    rdfs:subClassOf ids:Catalog;
    rdfs:label "App Resource Catalog"@en ;
    rdfs:comment "Class that aggregates App Resources , as a whole, from a (distributable) Catalog. May be used to list installed apps in a component."@en ;
    idsm:validation [
        idsm:forProperty ids:listedAppResource;
        idsm:relationType idsm:OneToMany;
    ];
.

ids:ClearingHouseCatalog
    rdfs:subClassOf ids:Catalog;
    a owl:Class;
    rdfs:label "Clearing House Catalog"@en ;
    rdfs:comment "Class that aggregates AppStores , as a whole, from a (distributable) Catalog."@en ;
    idsm:validation [
        idsm:forProperty ids:listedClearingHouse;
        idsm:relationType idsm:OneToMany;
    ];
.


# Properties
# ----------

ids:offeredResource a owl:ObjectProperty;
    rdfs:subPropertyOf dcat:dataset;
    rdfs:domain ids:ResourceCatalog;
    rdfs:range ids:Resource;
    rdfs:label "offered resource"@en;
    rdfs:comment "A Resource that is part of a resource catalog, indicating an offering (of, e.g., data)."@en.

ids:requestedResource a owl:ObjectProperty;
    rdfs:subPropertyOf dcat:dataset;
    rdfs:domain ids:ResourceCatalog;
    rdfs:range ids:Resource;
    rdfs:label "requested resource"@en;
    rdfs:comment "A Resource that is part of a resource catalog, indicating a request (of, e.g., data, software,...)."@en.

ids:member a owl:ObjectProperty;
    rdfs:subPropertyOf dcat:dataset;
    rdfs:domain ids:ParticipantCatalog;
    rdfs:range ids:Participant;
    rdfs:label "member"@en;
    rdfs:comment "A Participant, that is part of a participant catalog."@en.

ids:listedConnector a owl:ObjectProperty;
    rdfs:subPropertyOf dcat:dataset;
    rdfs:domain ids:ConnectorCatalog;
    rdfs:range ids:Connector;
    rdfs:label "listed Connector"@en;
    rdfs:comment "A Connector, that is part of a Connector catalog."@en;
.

ids:listedClearingHouse a owl:ObjectProperty;
   rdfs:subPropertyOf dcat:dataset;
   rdfs:domain ids:ClearingHouseCatalog;
   rdfs:range ids:ClearingHouse;
   rdfs:label "listed Clearing House"@en;
   rdfs:comment "A Clearing House, that is part of a Clearing House catalog."@en;
.

ids:listedAppResource a owl:ObjectProperty;
    rdfs:subPropertyOf dcat:dataset;
    rdfs:domain ids:AppResourceCatalog;
    rdfs:range ids:AppResource;
    rdfs:label "listed AppResource"@en;
    rdfs:comment "An AppResource that is part of an AppResourceCatalog."@en.
