@prefix owl: <http://www.w3.org/2002/07/owl#> .
@prefix rdf: <http://www.w3.org/1999/02/22-rdf-syntax-ns#> .
@prefix rdfs: <http://www.w3.org/2000/01/rdf-schema#> .
@prefix xsd: <http://www.w3.org/2001/XMLSchema#> .
@prefix dct: <http://purl.org/dc/terms/> .
@prefix ids: <https://w3id.org/ids/core/> .
@prefix idsm: <https://w3id.org/ids/metamodel/> .


# Classes
# -------

ids:Service a owl:Class;
	idsm:isAbstract true;
    rdfs:label "Service"@en;
    rdfs:comment "Service implements an Interface with regard to a communication Protocol."@en
    .
    
ids:DataService rdfs:subClassOf ids:Service ;
    a owl:Class;
    rdfs:label "DataService"@en;
    rdfs:comment "Service that processes, stores or otherwise handles data (in contrast to controlling machines etc.)"@en;
    idsm:validation [
        idsm:forProperty ids:binding;
        idsm:constraint idsm:NotNull;
    ].

# Properties for describing a DataService
# ---------------------------------------

ids:binding a owl:ObjectProperty;
    rdfs:domain ids:DataService;
    rdfs:range ids:ProtocolBinding;
    rdfs:label "binding"@en;
    rdfs:comment "Links to the protocol bindings which define how to technically invoke the Service."@en.

